src/passes/16.5-self_mini_c_coq/michelson_restrictions.ml
@@ -1,0 +1,28 @@
+open Errors
+open Simple_utils.Trace
+
+module I = Ligo_coq_ocaml.Compiler
+module Micheline = Tezos_micheline.Micheline
+
+(* TODO: make it shared *)
+type meta = Mini_c.meta
+type bynder_meta = Mini_c.binder_meta
+type base_type = (meta, string) Micheline.node
+type oty = (meta, base_type) I.ty
+type expr = (meta, base_type, Ligo_prim.Literal_value.t, (meta, string) Micheline.node) I.expr
+type binds = (meta, base_type, Ligo_prim.Literal_value.t, (meta, string) Micheline.node) I.binds
+type args = (meta, base_type, Ligo_prim.Literal_value.t, (meta, string) Micheline.node) I.args
+
+
+let self_in_lambdas ~raise : expr -> expr =
+  fun e ->
+    match e with
+    | I.E_lam (_, I.Binds (_, _, body), _) ->
+      let f = fun ~raise e -> match e with
+				| I.E_inline_michelson (_, _, [Micheline.Prim (_, "SELF", _, _)], _) ->
+           raise.error (bad_self_address Ligo_prim.Constant.C_SELF)
+				| _ -> e
+			in
+      let _self_in_lambdas : expr = Helpers.map_expr (f ~raise) body in
+      e
+    | _ -> e
