src/passes/16.5-self_mini_c_coq/uncurry.ml
@@ -1,0 +1,254 @@
+module I = Ligo_coq_ocaml.Compiler
+module Micheline = Tezos_micheline.Micheline
+module Coq = Ligo_coq_ocaml
+
+type meta = Mini_c.meta
+type bynder_meta = Mini_c.binder_meta
+type base_type = (meta, string) Micheline.node
+type ty = (meta, base_type) I.ty
+type expr = (meta, base_type, Ligo_prim.Literal_value.t, (meta, string) Micheline.node) I.expr
+type binds = (meta, base_type, Ligo_prim.Literal_value.t, (meta, string) Micheline.node) I.binds
+type args = (meta, base_type, Ligo_prim.Literal_value.t, (meta, string) Micheline.node) I.args
+
+let dummy_meta = Mini_c.dummy_meta
+
+(* return list tuples (lambda's meta, binding's meta, variable type), body and return type *)
+let rec uncurry_lambda (depth : int) (expr : expr) :
+          (meta * meta * ty) list * expr * ty option =
+  match expr with
+  | I.E_lam (m1, I.Binds (m2, [ta], body), ret_ty) when depth > 0 ->
+     let (vars, body, ret_ty') = uncurry_lambda (depth - 1) body in
+     let ret_ty = Option.first_some ret_ty' (Some ret_ty) in
+     ((m1, m2, ta) :: vars, body, ret_ty)
+  | _ -> ([], expr, None)
+
+
+(* let rec uncurry_arrow (depth : int) (type_ : ty) : ty list * ty = *)
+(*   match type_ with *)
+(*   | T_func (_, type1, type2) when depth > 0 -> *)
+(*     let (rest, type2) = uncurry_arrow (depth - 1) type2 in *)
+(*     (type1 :: rest, type2) *)
+(*   | _ -> ([], type_) *)
+
+(* TODO: ask about more than two arguments *)
+let rec uncurry_app (expr : expr) : expr * expr list =
+  match expr with
+  | E_app (_, I.Args_cons (_, a, I.Args_cons (_, f, I.Args_nil _))) ->
+    let (lamb, args') = uncurry_app f in
+    (lamb, a :: args')
+  | _ -> (expr, [])
+
+let curried_depth_in_lambda (rhs : expr) : int =
+  let (vars, _, _) = uncurry_lambda Int.max_value rhs in
+  List.length vars
+
+let isvar f x : bool =
+  match x with
+  | I.E_var (_, x) -> Coq.PeanoNat.Nat.eqb f x
+  | _ -> false
+
+(* Finding the usage of a function in an expression: we will look for
+   functions which are _only_ used in applications with a certain
+   fixed number of args. *)
+type usage =
+  | Application of int (* number of applied args *)
+  | Other
+  | Unused
+
+let combine_usage (u1 : usage) (u2 : usage) : usage =
+  match (u1, u2) with
+  | (Application d1, Application d2) ->
+    if d1 = d2
+    then u1
+    else Other
+  | (Other, _) -> Other
+  | (_, Other) -> Other
+  | (Unused, u2) -> u2
+  | (u1, Unused) -> u1
+
+let usages = List.fold_left ~f:combine_usage ~init:Unused
+
+let rec usage_in_expr (f : Coq.Datatypes.nat) (expr : expr) : usage =
+  let self = usage_in_expr f in
+  let self_binder = function
+    | I.Binds (_, tys, body) ->
+       usage_in_expr (Coq.Nat.add f (Coq.Datatypes.length tys)) body
+  in
+  let rec self_args = function
+    | I.Args_cons (_, x, xs) -> combine_usage (self x) (self_args xs)
+    | I.Args_nil (_) -> Unused
+  in
+  match expr with
+  (* interesting cases: *)
+  | I.E_var (_, x) ->
+    if Coq.PeanoNat.Nat.eqb f x
+    (* if we got here, f wasn't only used in applications *)
+    then Other
+    else Unused
+  | I.E_app _ ->
+    let (g, args) = uncurry_app expr in
+    let g =
+      if isvar f g
+      (* found an application of f *)
+      then Application (List.length args)
+      (* else g might be something weird which contains a usage of f,
+         e.g. if expr is ((if b then f else h) arg) *)
+      else self g in
+    usages (g :: List.map ~f:self args)
+
+  | I.E_deref (_, x) ->
+    if Coq.PeanoNat.Nat.eqb f x
+    then Other
+    else Unused
+  | I.E_assign (_, x, e) ->
+    if Coq.PeanoNat.Nat.eqb f x
+    then Other
+    else self e
+
+  (* everything else is boilerplate... *)
+  | I.E_literal _ | I.E_unit _ | I.E_raw_michelson _ ->
+    Unused
+  | I.E_lam (_, binder, _) ->
+    self_binder binder
+  | I.E_left (_, _t, e)  -> self e
+  | I.E_right (_, _t, e) -> self e
+  | I.E_failwith (_, e)  -> self e
+  | I.E_pair (_, args)   -> self_args args
+  | I.E_car (_, e)       -> self e
+  | I.E_cdr (_, e)       -> self e
+
+  | I.E_iter (_, v1, e1) ->
+    usages [self_binder v1; self e1]
+  | I.E_map (_, v1, e1) ->
+    usages [self_binder v1; self e1]
+  | I.E_loop_left (_, v1, _ty, e1) ->
+    usages [self_binder v1; self e1]
+  | I.E_fold (_, e1, e2, v1) ->
+    usages [self_binder v1; self e1; self e2]
+  | I.E_fold_right (_, _, e1, e2, v1) ->
+    usages [self_binder v1; self e1; self e2]
+
+  | I.E_if_bool (_, e1, e2, e3) ->
+    usages [self e1; self e2; self e3]
+  | I.E_if_none (_, e1, e2, v3) ->
+    usages [self e1; self e2; self_binder v3]
+  | I.E_if_cons (_, e1, vht, e2) ->
+    usages [self e1; self e2; self_binder vht]
+  | I.E_if_left (_, e1, v1, v2) ->
+    usages [self e1; self_binder v1; self_binder v2]
+
+  | I.E_let_in (_, e, binder) ->
+    usages [self e; self_binder binder]
+  | I.E_tuple (_, args) ->
+    self_args args
+  | I.E_let_tuple (_, e, vars) ->
+    usages [self e; self_binder vars]
+  | I.E_proj (_, e, _i, _n) ->
+    self e
+  | I.E_update (_, args, _i, _n) ->
+    self_args args
+  | I.E_inline_michelson (_, _, _, args) ->
+    self_args args
+  | I.E_global_constant (_, _ty, _hash, args) ->
+    self_args args
+  | I.E_create_contract (_, _p, _s, _code, args) -> (* TODO *)
+    self_args args
+
+  | I.E_let_mut_in (_, e, binder) ->
+    usages [self e; self_binder binder]
+  | I.E_for (_, e1, e2) ->
+    usages [self_args e1; self_binder e2]
+  | I.E_for_each (_, e1, e2) ->
+    usages [self e1; self_binder e2]
+  | I.E_while (_, e1, e2) ->
+    usages [self e1; self e2]
+
+let rec comb_type (ts : ty list) : ty =
+  match ts with
+  | x :: y :: [] -> I.T_pair (dummy_meta, None, None, x, y)
+  | x :: xs -> I.T_pair (dummy_meta, None, None, x, comb_type xs)
+  | [] -> I.T_unit (dummy_meta)
+
+(* let comb_expr (es : expr list) : expr = *)
+(*   I.E_tuple (dummy_meta, Helpers.args_of_list es) *)
+
+let uncurry_rhs (depth : int) (expr : expr) : expr * ty =
+  (*  λ x. λy. λ z. body => λ t. let (x, y) = t in λ z. body *)
+  (* Format.printf "\nUNCURRY_RHS:\n%a" Helpers.pp_expr expr; *)
+  let m = dummy_meta in
+  let (vars, body, ret_ty) = uncurry_lambda depth expr in
+  (* body save all binding and their order, but we need add one for new tuple
+     argument right before them *)
+  let body = Coq.Compiler.shift Helpers.nat_one (Coq.Datatypes.length vars) body in
+  let _, _, var_tys = List.unzip3 vars in
+  let arg_ty = comb_type var_tys in
+  let ret_ty = match ret_ty with Some ty -> ty | None -> assert false in
+
+  (* TODO: we can remove it by passing tuple in reverse order *)
+  let _, vs = List.fold_left vars ~init:(Coq.Datatypes.O, [])
+                  ~f:(fun (i, acc) (_, vm, vt) -> (S (S i),  (i, vm, vt) :: acc)) in
+  let vs = List.rev vs in (* because fold_left reverse [vs] *)
+  let body = Coq.Compiler.shift (Coq.Datatypes.length vars) (Coq.Datatypes.length vars) body in
+  let body = List.fold_right vs ~init:body
+                 ~f:(fun (vi, vm, vt) body ->
+                     I.E_let_in (m, I.E_var (m, vi), I.Binds (vm, [vt], body)))
+                 (* shift up all variables expect first [length vars] that is binded to arguments   *)
+  in
+  let binder_expr = I.E_var (m, Coq.Datatypes.O) in
+  (* TODO: Investigate how order of [var_tys] and tuple arguments correspond *)
+  let body = I.E_let_tuple (m, binder_expr, I.Binds (m, var_tys, body)) in
+  (* Format.printf "type: %a %a\n" Helpers.pp_ty (arg_ty) Helpers.pp_ty ret_ty; *)
+  let rsh = I.E_lam (Helpers.get_meta expr, I.Binds (m, [arg_ty], body), ret_ty) in
+  (* Format.printf "\nOUTPUT:\n%a\n\n" Helpers.pp_expr rsh; *)
+  let rsh_type = I.T_func (m, arg_ty, ret_ty) in
+  (rsh, rsh_type)
+
+(* hack to specialize map_expression to identity monad since there are
+   no errors here *)
+let map_expression = Helpers.map_expr
+let mapi_expression = Helpers.mapi_expr
+
+(* TODO: _depth *)
+let uncurry_in_expression
+    (f : Coq.Datatypes.nat) (_depth : int) : expr -> expr =
+  mapi_expression ~init:f
+    (fun f expr ->
+       (* Format.printf "\nUNCURRY_BODY (f = %a):\n%a\n\n" *)
+           (* Helpers.print_nat f Helpers.pp_expr expr; *)
+       let dummy = dummy_meta in
+       match expr with
+       | I.E_app (m, _) ->
+         let (lamb, args) = uncurry_app expr in
+         if isvar f lamb
+         then
+           (* the interesting part... *)
+           let arg_tuple = I.E_tuple (dummy, Helpers.args_of_list args) in
+           I.E_app (m, Helpers.args_of_list [arg_tuple; lamb])
+           (* let e' = I.E_app (m, Helpers.args_of_list [arg_tuple; lamb]) in *)
+           (* Format.printf "\nCHANGE to %a\n" Helpers.pp_expr e'; e' *)
+         else
+           expr
+       | _ -> expr)
+
+let uncurry_expression : expr -> expr =
+  map_expression
+    (fun e ->
+       match e with
+       | I.E_let_in (m1, e1, I.Binds (m2, ts, e2)) ->
+         let return e1 e1_ty e2 = I.E_let_in (m1, e1, I.Binds (m2, e1_ty, e2)) in
+         let depth_in_rhs = curried_depth_in_lambda e1 in
+         if depth_in_rhs > 0
+         then
+           match usage_in_expr Coq.Datatypes.O e2 with
+           | Unused | Other -> return e1 ts e2
+           | Application depth ->
+             if depth_in_rhs >= depth && depth > 1
+             then
+               let e1, e1_ty = uncurry_rhs depth e1 in
+               let e2 = uncurry_in_expression (Coq.Datatypes.O) depth e2 in
+               return e1 [e1_ty] e2
+             else
+               return e1 ts e2
+         else
+           e
+       | _ -> e)
