src/passes/predefined/predefined.ml
@@ -136,4 +136,137 @@ module Michelson = struct
         )
     | _ -> None
 
+  (* true if the name names a pure constant -- i.e. if uses will be pure
+     assuming arguments are pure *)
+  let is_pure_constant : constant' -> bool =
+    function
+    | C_UNIT
+    | C_CAR | C_CDR | C_PAIR
+    | C_NIL | C_CONS
+    | C_NEG | C_OR | C_AND | C_XOR | C_NOT
+    | C_EQ  | C_NEQ | C_LT | C_LE | C_GT | C_GE
+    | C_NONE | C_SOME
+    | C_LEFT | C_RIGHT
+    | C_TRUE | C_FALSE
+    | C_UPDATE | C_MAP_FIND_OPT | C_MAP_ADD | C_MAP_UPDATE
+    | C_ADDRESS
+    | C_CONCAT
+    | C_SET_MEM | C_SET_ADD | C_SET_REMOVE | C_SET_UPDATE
+    | C_LOOP_CONTINUE | C_LOOP_STOP
+    | C_SUB_MUTEZ
+    | C_BYTES_UNPACK
+    | C_SET_EMPTY | C_SET_LITERAL
+    | C_LIST_EMPTY | C_LIST_LITERAL
+    | C_MAP_EMPTY | C_MAP_LITERAL
+    | C_MAP_GET | C_MAP_REMOVE
+    | C_MAP_GET_AND_UPDATE | C_BIG_MAP_GET_AND_UPDATE
+    | C_BIG_MAP_EMPTY
+    | C_SAPLING_EMPTY_STATE
+    | C_SAPLING_VERIFY_UPDATE
+    | C_OPEN_CHEST
+    | C_GLOBAL_CONSTANT (* pure because restricted to PUSH *)
+    | C_EMIT_EVENT
+      -> true
+    (* unfortunately impure: *)
+    | C_ADD | C_SUB |C_MUL|C_DIV|C_MOD | C_LSL | C_LSR
+    | C_POLYMORPHIC_ADD | C_POLYMORPHIC_SUB
+    (* impure: *)
+    | C_UNOPT
+    | C_UNOPT_WITH_ERROR
+    | C_OPTION_MAP
+    | C_MAP_FIND
+    | C_CALL
+    | C_ITER
+    | C_LOOP_LEFT
+    | C_FOLD
+    | C_FOLD_LEFT
+    | C_FOLD_RIGHT
+    | C_SET_ITER
+    | C_SET_FOLD
+    | C_SET_FOLD_DESC
+    | C_LIST_ITER
+    | C_LIST_MAP
+    | C_LIST_FOLD
+    | C_LIST_FOLD_LEFT
+    | C_LIST_FOLD_RIGHT
+    | C_MAP_GET_FORCE
+    | C_MAP_ITER
+    | C_MAP_MAP
+    | C_MAP_FOLD
+    | C_SET_DELEGATE
+    | C_CREATE_CONTRACT
+    (* TODO? *)
+    | C_MAP
+    | C_BIG_MAP
+    | C_BIG_MAP_LITERAL
+    | C_CONTRACT
+    | C_CONTRACT_WITH_ERROR
+    | C_CONTRACT_OPT
+    | C_CONTRACT_ENTRYPOINT
+    | C_CONTRACT_ENTRYPOINT_OPT
+    | C_SELF
+    | C_SELF_ADDRESS
+    | C_IMPLICIT_ACCOUNT
+    | C_VIEW
+    (* Test - ligo interpreter, should never end up here *)
+    | C_TEST_SIZE
+    | C_TEST_ORIGINATE
+    | C_TEST_GET_STORAGE_OF_ADDRESS
+    | C_TEST_GET_BALANCE
+    | C_TEST_SET_SOURCE
+    | C_TEST_SET_BAKER
+    | C_TEST_EXTERNAL_CALL_TO_ADDRESS
+    | C_TEST_EXTERNAL_CALL_TO_ADDRESS_EXN
+    | C_TEST_GET_NTH_BS
+    | C_TEST_PRINT
+    | C_TEST_TO_STRING
+    | C_TEST_UNESCAPE_STRING
+    | C_TEST_STATE_RESET
+    | C_TEST_BOOTSTRAP_CONTRACT
+    | C_TEST_NTH_BOOTSTRAP_CONTRACT
+    | C_TEST_LAST_ORIGINATIONS
+    | C_TEST_MUTATE_CONTRACT
+    | C_TEST_MUTATE_VALUE
+    | C_TEST_SAVE_MUTATION
+    | C_TEST_RUN
+    | C_TEST_COMPILE_CONTRACT
+    | C_TEST_DECOMPILE
+    | C_TEST_TO_CONTRACT
+    | C_TEST_TO_ENTRYPOINT
+    | C_TEST_TO_TYPED_ADDRESS
+    | C_TEST_RANDOM
+    | C_TEST_GENERATOR_EVAL
+    | C_TEST_NTH_BOOTSTRAP_TYPED_ADDRESS
+    | C_TEST_COMPILE_CONTRACT_FROM_FILE
+    | C_TEST_COMPILE_AST_CONTRACT
+    | C_TEST_SET_BIG_MAP
+    | C_TEST_CAST_ADDRESS
+    | C_TEST_CREATE_CHEST
+    | C_TEST_CREATE_CHEST_KEY
+    | C_TEST_ADD_ACCOUNT
+    | C_TEST_NEW_ACCOUNT
+    | C_TEST_BAKER_ACCOUNT
+    | C_TEST_REGISTER_DELEGATE
+    | C_TEST_BAKE_UNTIL_N_CYCLE_END
+    | C_TEST_GET_VOTING_POWER
+    | C_TEST_GET_TOTAL_VOTING_POWER
+    | C_TEST_REGISTER_CONSTANT
+    | C_TEST_CONSTANT_TO_MICHELSON
+    | C_TEST_REGISTER_FILE_CONSTANTS
+    | C_TEST_PUSH_CONTEXT
+    | C_TEST_POP_CONTEXT
+    | C_TEST_DROP_CONTEXT
+    | C_TEST_FAILWITH
+    | C_TEST_READ_CONTRACT_FROM_FILE
+    | C_TEST_SIGN
+    | C_TEST_GET_ENTRYPOINT
+    | C_TEST_INT64_OF_INT
+    | C_TEST_INT64_TO_INT
+    | C_TEST_LAST_EVENTS
+    | C_TEST_TRY_WITH
+    | C_TEST_ABS
+    | C_TEST_INT
+    | C_TEST_SLICE
+      -> false
+
 end
